SimAsm/SimAsm.thy
@@ -10,14 +10,15 @@ fun re\<^sub>i :: "('v,'g,'r) op \<Rightarrow> ('v,'g,'r) op \<Rightarrow> bool"
     "re\<^sub>i (cmp b) \<alpha> = (\<alpha> \<noteq> full_fence \<and> wr \<alpha> \<subseteq> locals \<and> rd (cmp b) \<inter> wr \<alpha> = {} \<and> rd (cmp b) \<inter> rd \<alpha> \<subseteq> locals)" |
     "re\<^sub>i \<alpha> \<beta> = (\<beta> \<noteq> full_fence \<and> wr \<alpha> \<inter> wr \<beta> = {} \<and> rd \<alpha> \<inter> wr \<beta> = {} \<and> rd \<alpha> \<inter> rd \<beta> \<subseteq> locals)"
 
-fun re\<^sub>i' :: "('v,'g,'r) op \<Rightarrow> ('v,'g,'r) op \<Rightarrow> bool" where
-"re\<^sub>i' full_fence \<alpha> = False" |
-"re\<^sub>i' \<alpha> full_fence = False" |
-"re\<^sub>i' (cmp b) \<alpha> = ((wr \<alpha> \<subseteq> locals) \<and> (wr \<alpha> \<inter> rd (cmp b) = {}) \<and> (rd (cmp b) \<inter> rd \<alpha> \<subseteq> locals))" |
-"re\<^sub>i' \<alpha> \<beta> = ((wr \<alpha> \<inter> wr \<beta> = {}) \<and> (wr \<beta> \<inter> rd \<alpha> = {}) \<and> (rd \<alpha> \<inter> rd \<beta> \<subseteq> locals))"
+fun re\<^sub>i' :: "('v,'g,'r) op \<Rightarrow> ('v,'g,'r) op \<Rightarrow> bool" 
+  where
+    "re\<^sub>i' full_fence \<alpha> = False" |
+    "re\<^sub>i' \<alpha> full_fence = False" |
+    "re\<^sub>i' (cmp b) \<alpha> = ((wr \<alpha> \<subseteq> locals) \<and> (wr \<alpha> \<inter> rd (cmp b) = {}) \<and> (rd (cmp b) \<inter> rd \<alpha> \<subseteq> locals))" |
+    "re\<^sub>i' \<alpha> \<beta> = ((wr \<alpha> \<inter> wr \<beta> = {}) \<and> (wr \<beta> \<inter> rd \<alpha> = {}) \<and> (rd \<alpha> \<inter> rd \<beta> \<subseteq> locals))"
 
 lemma "re\<^sub>i' \<alpha> \<beta> = re\<^sub>i \<alpha> \<beta>"
-by (induction rule: re\<^sub>i'.induct) auto
+  by (induction rule: re\<^sub>i'.induct) auto
 
 fun fwd\<^sub>i  :: "('v,'g,'r) op \<Rightarrow> ('v,'g,'r) op \<Rightarrow> ('v,'g,'r) op" 
   where "fwd\<^sub>i \<alpha> (assign x e) = subst\<^sub>i \<alpha> x e" | "fwd\<^sub>i \<alpha> _ = \<alpha>"
@@ -33,7 +34,7 @@ This auxiliary state cannot influence real execution behaviour by definition.
 \<close>
 type_synonym ('v,'g,'r,'a) auxop = "('v,'g,'r) op \<times> ('v,'g,'r,'a) auxfn"
 
-fun beh\<^sub>a :: "('v,'g,'r,'a) auxop \<Rightarrow> ('v,'g,'r,'a) state rel"
+fun beh\<^sub>a :: "('v::truth,'g,'r,'a) auxop \<Rightarrow> ('v,'g,'r,'a) state rel"
   where "beh\<^sub>a (\<alpha>,f) = beh\<^sub>i \<alpha> O {(m,m'). m' = m(aux: f)}"
 
 fun re\<^sub>a :: "('v,'g,'r,'a) auxop \<Rightarrow> ('v,'g,'r,'a) auxop \<Rightarrow> bool" 
@@ -47,18 +48,18 @@ and behaviour in a tuple\<close>
 type_synonym ('v,'g,'r,'a) opbasic = "(('v,'g,'r,'a) auxop, ('v,'g,'r,'a) state) basic"
 
 text \<open>Duplicate forwarding and reordering behaviour of underlying instruction\<close>
-fun fwd\<^sub>s :: "('v,'g,'r,'a) opbasic \<Rightarrow> ('v,'g,'r,'a) auxop \<Rightarrow> ('v,'g,'r,'a) opbasic" 
+fun fwd\<^sub>s :: "('v::truth,'g,'r,'a) opbasic \<Rightarrow> ('v,'g,'r,'a) auxop \<Rightarrow> ('v,'g,'r,'a) opbasic" 
   where 
     "fwd\<^sub>s ((\<alpha>,f),v,b) (assign x e,_) = (let p = (subst\<^sub>i \<alpha> x e, f) in  (p,v, beh\<^sub>a p))" |
     "fwd\<^sub>s ((\<alpha>,f),v,b) (\<beta>,_) = ((\<alpha>,f),v,beh\<^sub>a (\<alpha>,f))"
 
 text \<open>Lift an operation with specification\<close>
-definition liftg :: "('v,'g,'r,'a) pred \<Rightarrow> ('v,'g,'r) op \<Rightarrow> ('v,'g,'r,'a) auxfn \<Rightarrow> ('v,'g,'r,'a) opbasic" 
+definition liftg :: "('v::truth,'g,'r,'a) pred \<Rightarrow> ('v,'g,'r) op \<Rightarrow> ('v,'g,'r,'a) auxfn \<Rightarrow> ('v,'g,'r,'a) opbasic" 
   ("\<lfloor>_,_,_\<rfloor>" 100)
   where "liftg v \<alpha> f \<equiv> ((\<alpha>,f), v, beh\<^sub>a (\<alpha>,f))"
 
 text \<open>Lift an operation without specification\<close>
-definition liftl :: "('v,'g,'r) op \<Rightarrow> ('v,'g,'r,'a) opbasic" 
+definition liftl :: "('v::truth,'g,'r) op \<Rightarrow> ('v,'g,'r,'a) opbasic" 
   ("\<lfloor>_\<rfloor>" 100)
   where "liftl \<alpha> \<equiv> ((\<alpha>,state_rec.more), UNIV, beh\<^sub>a (\<alpha>,state_rec.more))"
 
@@ -68,8 +69,8 @@ datatype ('v,'g,'r,'a) lang =
   Skip
   | Op "('v,'g,'r,'a) pred" "('v,'g,'r) op" "('v,'g,'r,'a) auxfn"
   | Seq "('v,'g,'r,'a) lang" "('v,'g,'r,'a) lang"
-  | If "('v,'g,'r) bexp" "('v,'g,'r,'a) lang" "('v,'g,'r,'a) lang"
-  | While "('v,'g,'r) bexp" "('v,'g,'r,'a) pred" "('v,'g,'r,'a) lang"
-  | DoWhile "('v,'g,'r,'a) pred" "('v,'g,'r,'a) lang" "('v,'g,'r) bexp"
+  | If "('v,'g,'r) exp" "('v,'g,'r,'a) lang" "('v,'g,'r,'a) lang"
+  | While "('v,'g,'r) exp" "('v,'g,'r,'a) pred" "('v,'g,'r,'a) lang"
+  | DoWhile "('v,'g,'r,'a) pred" "('v,'g,'r,'a) lang" "('v,'g,'r) exp"
 
 end
