Expression.thy
@@ -1,0 +1,98 @@
+theory Expression
+  imports Main 
+begin
+
+section \<open>Expression Language\<close>
+
+datatype ('v,'r) exp = 
+  Var 'r | 
+  Val 'v | 
+  Exp "'v list \<Rightarrow> 'v" "('v,'r) exp list"
+
+locale expression =
+  fixes lookup :: "'m \<Rightarrow> 'r \<Rightarrow> 'v"
+  fixes update :: "'m \<Rightarrow> 'r \<Rightarrow> 'v \<Rightarrow> 'm"
+  assumes lookup_update: "\<And>m r r' v. lookup (update m r v) r' = (if r = r' then v else lookup m r')"
+
+context expression
+begin
+
+definition Uop
+  where "Uop f i = Exp (\<lambda>l. case l of [v] \<Rightarrow> f v | _ \<Rightarrow> undefined) [i]"
+
+definition Bop
+  where "Bop f i j = Exp (\<lambda>l. case l of [v,v'] \<Rightarrow> f v v' | _ \<Rightarrow> undefined) [i,j]"
+
+text \<open>Evaluate an expression given a state\<close>
+fun eval :: "'m \<Rightarrow> ('v,'r) exp \<Rightarrow> 'v"
+  where 
+    "eval m (Var r) = lookup m r" |
+    "eval _ (Val v) = v" |
+    "eval m (Exp f rs) = f (map (eval m) rs)"
+
+text \<open>The syntactic dependencies of an expression\<close>
+fun deps :: "('v,'r) exp \<Rightarrow> 'r set"
+  where 
+    "deps (Var r) = {r}" |
+    "deps (Exp _ rs) = \<Union>(deps ` set rs)" |
+    "deps _ = {}"
+
+text \<open>Substitute a variable for an expression\<close>
+fun subst :: "('v,'r) exp \<Rightarrow> 'r \<Rightarrow> ('v,'r) exp \<Rightarrow> ('v,'r) exp"
+  where
+    "subst (Var r) r' e = (if r = r' then e else Var r)" |
+    "subst (Exp f rs) r e = (Exp f (map (\<lambda>x. subst x r e) rs))" |
+    "subst e _ _ = e"
+
+
+subsection \<open>Expression\<close>
+
+lemma eval_subst [simp]:
+  "eval m (subst e r f) = eval (update m r (eval m f)) e"
+proof (induct e)
+  case (Exp fn rs)
+  hence [simp]: "map (eval m \<circ> (\<lambda>x. subst x r f)) rs = map (eval (update m r (eval m f))) rs" 
+    by auto
+  show ?case by simp
+qed (auto simp: lookup_update)
+
+lemma eval_eq_state [intro]:
+  "\<forall>x \<in> deps e. lookup m x = lookup m' x \<Longrightarrow> eval m e = eval m' e"
+proof (induct e)
+  case (Exp fn rs)
+  hence [simp]: "map (eval m) rs = map (eval m') rs" by auto
+  thus ?case by simp
+qed auto
+
+lemma subst_nop [simp]:
+  "r \<notin> deps e \<Longrightarrow> subst e r f = e"
+proof (induct e)
+  case (Exp fn rs)
+  hence [simp]: "map (\<lambda>x. subst x r f) rs = rs" by (induct rs) auto
+  show ?case by simp
+qed auto
+
+lemma deps_subst [simp]:
+  "deps (subst e x e') = deps e - {x} \<union> (if x \<in> deps e then deps e' else {})"
+  by (induct e; auto simp: if_splits)
+
+lemma finite_deps [intro]:
+  "finite (deps e)"
+  by (induct e) auto
+
+lemma subst_fp [simp]:
+  "subst (subst e x (Val v')) x (Val v) = subst e x (Val v')"
+  by (induct e) auto
+
+lemma subst_flip [simp]:
+  "x \<noteq> y \<Longrightarrow> subst (subst e x (Val v')) y (Val v) = subst (subst e y (Val v)) x (Val v')"
+  by (induct e) auto
+
+end
+
+class truth =
+  fixes holds :: "'a \<Rightarrow> bool"
+  fixes neg :: "'a \<Rightarrow> 'a"
+  assumes inv: "holds (neg a) \<equiv> \<not> holds a"
+
+end
